Properly instantiate Blocks (see Types.v)

Extraction/src/Util.ml
@@ -1,0 +1,18 @@
+open Forests
+
+module Types = Impl.TypesImpl
+module ConsensusParams = Impl.ProofOfWork
+module ForestImpl = Forests (Types) (ConsensusParams)
+
+open Types
+
+let string_of_tx = string_of_int
+
+let string_of_block (b : coq_Block) =
+  let fmt = format_of_string "{prev = %s, txs = %s}" in
+  Printf.sprintf fmt
+    (string_of_int b.prevBlockHash)
+    (String.concat " " (List.map string_of_tx b.txs))
+
+let string_of_blockchain (chain : coq_Blockchain) =
+  String.concat " " (List.map string_of_block chain)
