Extraction/src/node.ml
@@ -3,9 +3,10 @@ open Protocol
 open Util
 
 module Addr = Address.Addr
+module Types = Impl.TypesImpl
 module ConsensusParams = Impl.ProofOfWork
-module ForestImpl = Forests (ConsensusParams)
-module ProtocolImpl = Protocol (ConsensusParams) (ForestImpl) (Addr)
+module ForestImpl = Forests (Types) (ConsensusParams)
+module ProtocolImpl = Protocol (Types) (ConsensusParams) (ForestImpl) (Addr)
 
 let node_id = 0
 let st = ref (ProtocolImpl.coq_Init node_id);;
@@ -13,13 +14,14 @@ let st = ref (ProtocolImpl.coq_Init node_id);;
 open ForestImpl
 
 let main () =
-  let argv = Array.to_list Sys.argv in
-  let args = List.tl argv in
+  let chain = btChain !st.blockTree in
+  Printf.printf "Chain: %s\n" (string_of_blockchain chain) ;;
+
   let blocks = all_blocks !st.blockTree in
   Printf.printf "Your blocktree has %s block(s)!\n"
     (string_of_int (List.length blocks)) ;;
+ 
   Printf.printf "You are node %s\n" (string_of_int !st.id) ;;
-
 
 let () = main ()
 
